more 3.6

analysis/Analysis/Section_3_6.lean
@@ -96,6 +96,42 @@ theorem SetTheory.Set.has_card_iff (X:Set) (n:ℕ) :
     X.has_card n ↔ ∃ f: X → Fin n, Function.Bijective f := by
   simp [has_card, HasEquiv.Equiv, Setoid.r, EqualCard]
 
+abbrev SetTheory.Set.singleton_has_card (x: Object) : ({x}: Set).has_card 1 := by
+  rw [has_card_iff]
+  refine ⟨fun _ => Fin_mk 1 0 Nat.one_pos, ?_, ?_⟩
+  · intro a b h; clear h
+    rw [← coe_inj, mem_singleton _ _ |>.mp a.prop, mem_singleton _ _ |>.mp b.prop]
+  · intro n
+    obtain ⟨m, hm, hnm⟩ := mem_Fin _ _ |>.mp n.prop
+    replace hnm : (n: ℕ) = m := (Fin.coe_eq_iff n).mp hnm
+    obtain rfl : m = 0 := Nat.lt_one_iff.mp hm
+    refine ⟨⟨x, mem_singleton _ _ |>.mpr rfl⟩, ?_⟩ 
+    simp [hnm]
+
+abbrev SetTheory.Set.pair_has_card {x y: Object} (hxy : x ≠ y) : ({x, y}: Set).has_card 2 := by
+  rw [has_card_iff]
+  refine ⟨fun z => by
+    if z.val = x then exact Fin_mk 2 0 Nat.zero_lt_two
+    else exact Fin_mk 2 1 Nat.one_lt_two, ?_, ?_
+  ⟩
+  · intro a b h
+    simp at h
+    by_cases ha : a.val = x
+    <;> by_cases hb : b.val = x
+    · simpa [←hb, coe_inj] using ha
+    · simp [if_pos ha, if_neg hb] at h
+    · simp [if_neg ha, if_pos hb] at h
+    replace ha : a.val = y := mem_pair _ _ _ |>.mp a.prop |>.elim (ha · |>.elim) id
+    replace hb : b.val = y := mem_pair _ _ _ |>.mp b.prop |>.elim (hb · |>.elim) id
+    · simpa [←hb, coe_inj] using ha
+  · intro ⟨m, hm'⟩
+    obtain ⟨m, hm, rfl⟩ := mem_Fin _ _ |>.mp hm'
+    obtain (rfl|rfl) : m = 0 ∨ m = 1 := 
+      Nat.le_one_iff_eq_zero_or_eq_one.mp (Nat.le_of_lt_succ hm)
+    · exact ⟨⟨x, mem_pair _ _ _ |>.mpr (Or.inl rfl)⟩, by simp⟩
+    refine ⟨⟨y, mem_pair _ _ _ |>.mpr (Or.inr rfl)⟩, ?_⟩
+    simp [hxy.symm]
+
 /-- Remark 3.6.6 -/
 theorem SetTheory.Set.Remark_3_6_6 (n:ℕ) :
   (nat.specify (fun x ↦ 1 ≤ (x:ℕ) ∧ (x:ℕ) ≤ n)).has_card n := by
@@ -187,9 +223,6 @@ theorem SetTheory.Set.has_card_zero {X:Set} : X.has_card 0 ↔ X = ∅ := by
       exact (not_mem_empty _) (h ▸ hx) |>.elim
     · intro ⟨_, hx⟩
       exact (not_mem_empty _) (hFin_0 ▸ hx) |>.elim
-
-example : (n: ℕ) - p - q = n - q - p := by exact Nat.sub_right_comm n p q
-/- example : (n: ℕ) ≤ m → 0 ≤ m - n := by  -/
 
 /-- Lemma 3.6.9 -/
 theorem SetTheory.Set.card_erase {n:ℕ} (hn: n ≥ 1) {X:Set} (hX: X.has_card n) (x:X) :
@@ -401,6 +434,11 @@ theorem SetTheory.Set.has_card_to_card {X:Set} {n: ℕ}: X.has_card n → X.card
 
 theorem SetTheory.Set.card_to_has_card {X:Set} {n: ℕ} (hn: n ≠ 0): X.card = n → X.has_card n
   := by grind [card, has_card_card]
+
+theorem SetTheory.Set.card_to_has_card' {X:Set} {n: ℕ} (hX: X.finite) (hX_card: X.card = n) : X.has_card n := by
+  unfold card at hX_card
+  rw [← hX_card, dif_pos hX]
+  exact hX.choose_spec
 
 theorem SetTheory.Set.card_fin_eq (n:ℕ): (Fin n).has_card n := (has_card_iff _ _).mp ⟨ id, Function.bijective_id ⟩
 
@@ -771,55 +809,418 @@ theorem SetTheory.Set.card_prod {X Y:Set} (hX: X.finite) (hY: Y.finite) :
       Nat.succ_mul]
 
 noncomputable def SetTheory.Set.pow_fun_equiv {A B : Set} : ↑(A ^ B) ≃ (B → A) where
-  toFun x := sorry
-  invFun x := sorry
-  left_inv := sorry
-  right_inv := sorry
+  toFun := fun x => powerset_axiom _ |>.mp x.prop |>.choose
+  invFun := fun x => ⟨coe_of_fun x, powerset_axiom _ |>.mpr ⟨x, rfl⟩⟩
+  left_inv x := by
+    generalize_proofs _ h
+    simp [h x |>.choose_spec]
+  right_inv x := by simp
 
 lemma SetTheory.Set.pow_fun_eq_iff {A B : Set} (x y : ↑(A ^ B)) : x = y ↔ pow_fun_equiv x = pow_fun_equiv y := by
   rw [←pow_fun_equiv.apply_eq_iff_eq]
 
+theorem SetTheory.Set.empty_pow (hX : X ≠ empty) : empty ^ X = empty := by
+  ext x
+  simp
+  intro f
+  exact (not_mem_empty _) (f (nonempty_choose hX)).prop |>.elim
+
+@[simp]
+theorem SetTheory.Set.pow_empty {Y : Set} : 
+  Y ^ empty = {coe_of_fun (X := empty) (Y := Y) fun x => (not_mem_empty _) x.prop |>.elim} := by
+  simp [Set.ext_iff]
+  refine fun f => ⟨?_, ?_⟩ 
+  · rintro ⟨f, rfl⟩ 
+    rw [coe_of_fun_inj]
+    ext x
+    exact (not_mem_empty _) x.prop |>.elim
+  · exact fun h => by simp [h]
+
+example {a b: Prop} (h: ¬a) : a ∨ b ↔ b := or_iff_right h
+example {f g: α → β} (h: (fun x => f x) = fun x => g x) : f y = g y  := by exact congrFun h y
+
 /-- Proposition 3.6.14 (f) / Exercise 3.6.4 -/
 theorem SetTheory.Set.card_pow {X Y:Set} (hY: Y.finite) (hX: X.finite) :
-    (Y ^ X).finite ∧ (Y ^ X).card = Y.card ^ X.card := by sorry
+    (Y ^ X).finite ∧ (Y ^ X).card = Y.card ^ X.card := by
+    suffices (Y ^ X).has_card (Y.card ^ X.card) from ⟨⟨_, this⟩, has_card_to_card this⟩
+    apply induction_insert hX
+    · rw [pow_empty, empty_card_eq_zero, pow_zero]; exact singleton_has_card _
+    intro x X hX hx ih
+    rw [card_insert hX hx |>.right, pow_succ]
+    have : ((Y ^ X) ×ˢ Y).has_card (Y.card ^ X.card * Y.card) := by
+      have := card_prod ⟨_, ih⟩ hY
+      apply card_to_has_card' this.left
+      rw [this.right, has_card_to_card ih]
+    apply Setoid.trans ?_ this
+    let x': (X ∪ {x}).toSubtype := ⟨x, mem_union _ _ _ |>.mpr (Or.inr <| mem_singleton _ _ |>.mpr rfl)⟩
+    refine ⟨fun z =>
+      mk_cartesian (pow_fun_equiv.symm fun x => 
+        (pow_fun_equiv z ⟨x, mem_union _ _ _ |>.mpr (Or.inl x.prop)⟩)
+      ) (pow_fun_equiv z x')
+    , ?_, ?_⟩
+    · intro a b h
+      simp [mk_cartesian, coe_inj] at h
+      apply Equiv.injective pow_fun_equiv
+      ext y
+      by_cases hy : y.val ∈ X 
+      · replace h := congrFun h.left ⟨y, hy⟩
+        exact congrArg Subtype.val h
+      · have : y.val = x := mem_union _ _ _ |>.mp y.prop |> (or_iff_right hy).mp |> (mem_singleton _ _).mp
+        exact (coe_inj _ y x').mp this ▸ h.right ▸ rfl
+    · intro ⟨_, h⟩
+      obtain ⟨yx, y, rfl⟩ := mem_cartesian _ _ _ |>.mp h
+      use pow_fun_equiv.symm fun x' => by
+        if h : x'.val ∈ X then exact pow_fun_equiv yx ⟨x', h⟩ 
+        else exact y
+      simp [mk_cartesian, coe_inj]
+      constructor
+      · apply pow_fun_equiv.injective
+        ext x
+        rw [Equiv.apply_symm_apply, if_pos x.prop]
+      · exact fun h ↦ (hx h).elim
 
 /-- Exercise 3.6.5. You might find `SetTheory.Set.prod_commutator` useful. -/
 theorem SetTheory.Set.prod_EqualCard_prod (A B:Set) :
-    EqualCard (A ×ˢ B) (B ×ˢ A) := by sorry
+  EqualCard (A ×ˢ B) (B ×ˢ A) := by
+    use prod_commutator A B
+    exact Equiv.bijective (A.prod_commutator B)
 
 noncomputable abbrev SetTheory.Set.pow_fun_equiv' (A B : Set) : ↑(A ^ B) ≃ (B → A) :=
   pow_fun_equiv (A:=A) (B:=B)
 
+def EquivReturn {A B C: Sort*} (b_equiv_c: B ≃ C) : (A → B) ≃ (A → C) where
+  toFun f a := b_equiv_c (f a)
+  invFun f a := b_equiv_c.symm (f a)
+  left_inv f := by simp
+  right_inv f := by simp
+
+def EquivSwapArgs {A B C: Sort*} : (A → B → C) ≃ (B → A → C) where
+  toFun f b a := f a b
+  invFun f a b := f b a
+  left_inv _ := rfl
+  right_inv _ := rfl
+
 /-- Exercise 3.6.6. You may find `SetTheory.Set.curry_equiv` useful. -/
 theorem SetTheory.Set.pow_pow_EqualCard_pow_prod (A B C:Set) :
-    EqualCard ((A ^ B) ^ C) (A ^ (B ×ˢ C)) := by sorry
+  EqualCard ((A ^ B) ^ C) (A ^ (B ×ˢ C)) := by
+    use pow_fun_equiv' (A ^ B) C 
+      |>.trans (EquivReturn (pow_fun_equiv' A B))
+      |>.trans EquivSwapArgs 
+      |>.trans curry_equiv
+      |>.trans pow_fun_equiv.symm
+    exact Equiv.bijective _
 
-theorem SetTheory.Set.pow_pow_eq_pow_mul (a b c:ℕ): (a^b)^c = a^(b*c) := by sorry
+
+theorem SetTheory.Set.pow_pow_eq_pow_mul (a b c:ℕ): (a^b)^c = a^(b*c) := by
+  have hA_B := card_pow (Fin_finite a) (Fin_finite b)
+  have hA_B_C := card_pow hA_B.left (Fin_finite c)
+  have hBC := card_prod (Fin_finite b) (Fin_finite c)
+  have hA_BC := card_pow (Fin_finite a) hBC.left
+  rw [
+    ← Fin_card a, ← Fin_card b, ← Fin_card c, 
+    ← hA_B.right, ← hA_B_C.right, 
+    ← hBC.right, ← hA_BC.right, 
+    EquivCard_to_card_eq]
+  exact pow_pow_EqualCard_pow_prod _ _ _
 
 theorem SetTheory.Set.pow_prod_pow_EqualCard_pow_union (A B C:Set) (hd: Disjoint B C) :
-    EqualCard ((A ^ B) ×ˢ (A ^ C)) (A ^ (B ∪ C)) := by sorry
+  EqualCard ((A ^ B) ×ˢ (A ^ C)) (A ^ (B ∪ C)) := by
+    replace hd: ∀x, x ∈ C → x ∉ B := by 
+      rw [disjoint_comm] at hd
+      simpa [disjoint_iff, eq_empty_iff_forall_notMem] using hd
+    refine ⟨fun a => by
+      have fb := pow_fun_equiv (fst a)
+      have fc := pow_fun_equiv (snd a)
+      exact pow_fun_equiv.symm fun bc => by
+        if hbc: bc.val ∈ B then 
+          exact fb ⟨bc, hbc⟩
+        else 
+          replace hbc := mem_union _ _ _ |>.mp bc.prop |>.elim
+            (fun h => hbc h |>.elim)
+            (fun h => h)
+          exact fc ⟨bc, hbc⟩
+      , ?_, ?_⟩
+    · intro ⟨a,ha⟩ ⟨b,hb⟩ h
+      obtain ⟨a1, a2, rfl⟩ := mem_cartesian _ _ _ |>.mp ha
+      obtain ⟨b1, b2, rfl⟩ := mem_cartesian _ _ _ |>.mp hb
+      simp [coe_inj] at ⊢ h
+      have h1 : pow_fun_equiv a1 = pow_fun_equiv b1 := by
+        ext b
+        have : b.val ∈ (B ∪ C) := mem_union _ _ _ |>.mpr (Or.inl b.prop)
+        replace h := congrArg (· ⟨b, this⟩) h
+        simp [dif_pos b.prop] at h
+        rw [h]
+      have h2 : pow_fun_equiv a2 = pow_fun_equiv b2 := by
+        ext c
+        have : c.val ∈ (B ∪ C) := mem_union _ _ _ |>.mpr (Or.inr c.prop)
+        replace h := congrArg (· ⟨c, this⟩) h
+        simp [dif_neg <| hd _ c.prop] at h
+        rw [h]
+      simp [h1, h2, pow_fun_eq_iff]
+    · intro ⟨f, hf⟩
+      obtain ⟨f, rfl⟩ := powerset_axiom _ |>.mp hf
+      let fb (b: B): A := f ⟨b, mem_union _ _ _ |>.mpr (Or.inl b.prop)⟩
+      let fc (c: C): A := f ⟨c, mem_union _ _ _ |>.mpr (Or.inr c.prop)⟩
+      use mk_cartesian (pow_fun_equiv.symm fb) (pow_fun_equiv.symm fc)
+      simp [pow_fun_equiv]
+      funext bc
+      generalize_proofs hfb hfc
+      split_ifs with h'
+      · rw [coe_of_fun_inj _ _ |>.mp hfb.choose_spec]
+      · rw [coe_of_fun_inj _ _ |>.mp hfc.choose_spec]
 
-theorem SetTheory.Set.pow_mul_pow_eq_pow_add (a b c:ℕ): (a^b) * a^c = a^(b+c) := by sorry
+theorem SetTheory.Set.pow_mul_pow_eq_pow_add (a b c:ℕ): (a^b) * a^c = a^(b+c) := by
+  let B := (Fin b).replace (P := fun b y => ((b: ℕ) + c: Object) = y) (by simp)
+  have mem_B (b': Fin b) : ((b': ℕ) + c: Object) ∈ B := replacement_axiom _ _ |>.mpr ⟨b', rfl⟩
+  have disj_B_C : Disjoint B (Fin c) := by
+    rw [disjoint_iff, inter_comm, eq_empty_iff_forall_notMem]
+    intro x
+    rw [mem_inter, not_and, mem_Fin]
+    rintro ⟨x, hx, rfl⟩
+    simp [B]
+    intro y hy h
+    obtain ⟨y, rfl⟩ : ∃n: ℕ, y = ↑n := ⟨(Subtype.mk y hy : ℕ), Object.ofnat_eq'' ▸ rfl⟩
+    simp at h
+    omega
+  have B_card : B.has_card b := by
+    apply Setoid.symm
+    refine ⟨fun b => ⟨_, mem_B b⟩, ?_, ?_⟩
+    · intro x y h
+      simpa [coe_inj] using h
+    · intro x
+      obtain ⟨b', hb'⟩ := replacement_axiom _ _ |>.mp x.prop
+      have : x = ⟨↑(↑b' + c), hb' ▸ x.prop⟩ := coe_inj _ _ _ |>.mp hb'.symm
+      simp [this]
+  have hA_B := card_pow (Fin_finite a) ⟨_, B_card⟩
+  have hA_C := card_pow (Fin_finite a) (Fin_finite c)
+  have hA_B_C := card_pow hA_B.left (Fin_finite c)
+  rw [
+    ← Fin_card a, ← has_card_to_card B_card, ← Fin_card c, 
+    ← hA_B.right, ← hA_C.right, ← (card_prod hA_B.left hA_C.left).right,
+    ← card_union_disjoint ⟨_, B_card⟩ (Fin_finite c) disj_B_C,
+    ← card_pow (Fin_finite a) (card_union ⟨_, B_card⟩ (Fin_finite c)).left |>.right,
+    EquivCard_to_card_eq]
+  exact pow_prod_pow_EqualCard_pow_union _ _ _ disj_B_C
 
 /-- Exercise 3.6.7 -/
 theorem SetTheory.Set.injection_iff_card_le {A B:Set} (hA: A.finite) (hB: B.finite) :
-    (∃ f:A → B, Function.Injective f) ↔ A.card ≤ B.card := sorry
+  (∃ f:A → B, Function.Injective f) ↔ A.card ≤ B.card := by
+    constructor
+    · intro ⟨f, hf⟩
+      rw [← card_image_inj hA hf]
+      apply card_subset hB (image_in_codomain _ _) |>.right
+    intro h
+    obtain ⟨n, hn⟩ := hA
+    obtain rfl := has_card_to_card hn
+    obtain ⟨f, hf⟩ := hn
+    obtain ⟨m, hm⟩ := hB
+    obtain rfl := has_card_to_card hm
+    obtain ⟨g, hg⟩ := hm
+    refine ⟨fun a => Fin_embed A.card B.card h (f a) |> hg.surjective |>.choose, ?_⟩
+    intro x y h
+    simp at h
+    generalize_proofs hx hy at h
+    have := hy.choose_spec
+    rw [← h, hx.choose_spec, ← Fin.coe_inj] at this
+    exact hf.injective this
+
+theorem SetTheory.Set.empty_inter (A: Set) : ∅ ∩ A = ∅ := by simp [Set.ext_iff]
+
+theorem SetTheory.Set.empty_sdiff (A: Set) : ∅ \ A = ∅ := by simp [Set.ext_iff]
 
 /-- Exercise 3.6.8 -/
 theorem SetTheory.Set.surjection_from_injection {A B:Set} (hA: A ≠ ∅) (f: A → B)
-  (hf: Function.Injective f) : ∃ g:B → A, Function.Surjective g := by sorry
+  (hf: Function.Injective f) : ∃ g:B → A, Function.Surjective g := by
+    have : Nonempty A := ⟨nonempty_choose hA⟩
+    refine ⟨Function.invFun f, fun a => ⟨f a, ?_⟩⟩
+    exact hf Function.apply_invFun_apply
+
+theorem SetTheory.Set.inter_finite {A B:Set} (hA: A.finite)
+  : (A ∩ B).finite := by
+    apply induction_insert hA
+    · simp [empty_inter]
+    intro x X hX hx ih
+    rw [show ((X ∪ {x}) ∩ B) = X ∩ B ∪ {x} ∩ B by simp [Set.ext_iff]; tauto]
+    refine card_union ih ?_ |>.left
+    by_cases h: x ∈ B
+    · rw [show {x} ∩ B = {x} by simp [Set.ext_iff]; tauto]
+      exact ⟨_, singleton_has_card _⟩
+    · rw [show {x} ∩ B = ∅ by simp [Set.ext_iff]; tauto]
+      exact finite_of_empty rfl
+
+theorem SetTheory.Set.sdiff_finite {A B:Set} (hA: A.finite)
+  : (A \ B).finite := by
+    apply induction_insert hA
+    · simp [empty_sdiff]
+    intro x X hX hx ih
+    rw [show ((X ∪ {x}) \ B) = X \ B ∪ {x} \ B by simp [Set.ext_iff]; tauto]
+    refine card_union ih ?_ |>.left
+    by_cases h: x ∈ B
+    · rw [show {x} \ B = ∅ by simp [Set.ext_iff]; tauto]
+      exact finite_of_empty rfl
+    · rw [show {x} \ B = {x} by simp [Set.ext_iff]; tauto]
+      exact ⟨_, singleton_has_card _⟩
+
+theorem SetTheory.Set.partition_sdiff_inter (A B: Set) : A = A \ B ∪ A ∩ B := by 
+    simp [Set.ext_iff, ← and_or_left]
+    exact fun _ _ => or_comm.eq ▸ Classical.em _
+
+theorem SetTheory.Set.disjoint_union {A B C: Set} 
+  (hAC: Disjoint A C) (hBC: Disjoint B C) : Disjoint (A ∪ B) C := by
+    rw [disjoint_iff] at *
+    rw [show (A ∪ B) ∩ C = (A ∩ C) ∪ (B ∩ C) by simp [Set.ext_iff]; tauto, hAC, hBC, empty_union]
 
 /-- Exercise 3.6.9 -/
 theorem SetTheory.Set.card_union_add_card_inter {A B:Set} (hA: A.finite) (hB: B.finite) :
-    A.card + B.card = (A ∪ B).card + (A ∩ B).card := by  sorry
+    A.card + B.card = (A ∪ B).card + (A ∩ B).card := by 
+    nth_rw 1 [union_eq_partition, partition_sdiff_inter B A, partition_sdiff_inter A B]
+    rw [
+      card_union_disjoint (sdiff_finite hB) (inter_finite hB) disjoint_sdiff_inter,
+      inter_comm B A,
+      card_union_disjoint (card_union (sdiff_finite hA) (inter_finite hA)).left (sdiff_finite hB),
+      add_assoc
+    ]
+    refine disjoint_union disjoint_sdiff_sdiff ?_
+    rw [disjoint_comm, inter_comm]
+    exact disjoint_sdiff_inter
+
+theorem SetTheory.Set.iUnion_union {I I' J: Set} {A} (hJ: J = I ∪ I'):
+  J.iUnion A = I.iUnion (fun i => A ⟨i.val, hJ ▸ mem_union _ _ _ |>.mpr (Or.inl i.prop)⟩) ∪
+    I'.iUnion (fun i => A ⟨i.val, hJ ▸ mem_union _ _ _ |>.mpr (Or.inr i.prop)⟩) := by
+    ext x
+    simp only [mem_iUnion, mem_union]
+    constructor
+    · rintro ⟨⟨i, hi⟩, hx⟩
+      by_cases hj : i ∈ I
+      · refine Or.inl ⟨⟨i, hj⟩, ?_⟩
+        simpa
+      replace hj : i ∈ I' := mem_union _ _ _ |>.mp (hJ ▸ hi) |>.elim (hj · |>.elim) id
+      refine Or.inr ⟨⟨i, hj⟩, ?_⟩
+      simpa
+    rintro (⟨⟨j, hj⟩, hx⟩|⟨⟨j, hj⟩, hx⟩)
+    · exact ⟨⟨j, hJ ▸ mem_union _ _ _ |>.mpr (Or.inl hj)⟩, hx⟩
+    · exact ⟨⟨j, hJ ▸ mem_union _ _ _ |>.mpr (Or.inr hj)⟩, hx⟩
+
+theorem SetTheory.Set.iUnion_singleton {x: Object} {A} :
+    iUnion {x} A = A ⟨x, mem_singleton _ _ |>.mpr rfl⟩ := by
+      ext y
+      rw [mem_iUnion]
+      constructor
+      · rintro ⟨⟨x, hx⟩, ha⟩
+        exact (mem_singleton _ _ |>.mp hx) ▸ ha
+      exact fun ha => ⟨⟨x, mem_singleton _ _ |>.mpr rfl⟩, ha⟩
+
+theorem SetTheory.Set.iUnion_finite {I: Set} (hI: I.finite) {A : I → Set}  (hA: ∀ i, (A i).finite) :
+  (I.iUnion A).finite := by
+    revert A; apply induction_insert hI
+    · intro A; simp [iUnion_of_empty]
+    intro x X hX hx ih A hA
+    simp [iUnion_union rfl]
+    apply card_union (ih ?_) ?_ |>.left
+    · intro ⟨i, hi⟩
+      simp [hA ⟨i, mem_union _ _ _ |>.mpr (Or.inl hi)⟩]
+    simp [iUnion_singleton, hA ⟨x, mem_union _ _ _ |>.mpr (Or.inr <| mem_singleton _ _ |>.mpr rfl)⟩]
 
 /-- Exercise 3.6.10 -/
 theorem SetTheory.Set.pigeonhole_principle {n:ℕ} {A: Fin n → Set}
-  (hA: ∀ i, (A i).finite) (hAcard: (iUnion _ A).card > n) : ∃ i, (A i).card ≥ 2 := by sorry
+  (hA: ∀ i, (A i).finite) (hAcard: (iUnion _ A).card > n) : ∃ i, (A i).card ≥ 2 := by
+    induction' n with n ih
+    · have : Fin 0 = ∅ := has_card_zero.mp (Setoid.refl _)
+      simp [this ▸ iUnion_of_empty, this] at hAcard
+    let n' := (Fin_mk n.succ n (lt_add_one _))
+    by_cases hn_card : (A n').card ≥ 2
+    · exact ⟨n', hn_card⟩
+    replace hn_card : (A n').card = 0 ∨ (A n').card = 1  := by
+      have : (A n').card < 2 := by exact Nat.lt_of_not_le hn_card
+      replace : (A n').card ≤ 1 := by exact Nat.le_of_lt_succ this
+      exact Nat.le_one_iff_eq_zero_or_eq_one.mp this
+    let A' (n': Fin n): Set := A (Fin_embed n n.succ (Nat.le_succ n) n')
+    have hA' : ∀ i, (A' i).finite := by simp [A', hA]
+    have : Fin n.succ = (Fin n) ∪ {(n: Object)} := by
+      simp only [Nat.succ_eq_add_one, Set.ext_iff, mem_union, mem_singleton, mem_Fin]
+      have (x y: ℕ) : (x: Object) = (y: Object) → x = y := by 
+        exact fun a ↦ (fun [SetTheory] n m ↦ (ofNat_inj' n m).mp) x y a
+      intro x
+      constructor
+      · rintro ⟨m, hm, rfl⟩
+        by_cases hm_eq : m = n
+        · simp [hm_eq]
+        refine Or.inl ⟨m, ?_, rfl⟩
+        exact Nat.lt_of_le_of_ne (Nat.le_of_lt_succ hm) hm_eq
+      · rintro (⟨m, hm, rfl⟩|rfl) <;> simp
+        exact hm.le
+    have hA'card := hAcard
+    rw [iUnion_union this] at hA'card
+    replace hA'card := lt_of_lt_of_le hA'card (card_union 
+      (iUnion_finite (Fin_finite n) fun i => hA (Fin_embed n n.succ (Nat.le_succ _) i))
+      (iUnion_finite ⟨_, singleton_has_card _⟩ fun ⟨x, hx⟩ => 
+        have := mem_singleton _ _ |>.mp hx
+        hA ⟨x, mem_Fin _ _ |>.mpr ⟨n, lt_add_one n, this⟩⟩)
+      ).right
+    replace hA'card : n  < ((Fin n).iUnion fun i ↦ A (Fin_embed n n.succ (Nat.le_succ _) i)).card := by
+      rcases hn_card with hn|hn
+      · rw [iUnion_singleton, hn] at hA'card
+        exact lt_of_le_of_lt (Nat.le_succ _) hA'card
+      · rw [iUnion_singleton, hn] at hA'card
+        exact Nat.succ_lt_succ_iff.mp hA'card
+    obtain ⟨i, hi⟩ := ih hA' hA'card
+    exact ⟨Fin_embed n n.succ (Nat.le_succ _) i, hi⟩
+
+theorem SetTheory.Set.sdiff_of_singleton_mem {X Y: Set} {x: X} (hX: X \ {x.val} = Y) : Y ∪ {x.val} = X := by
+  simp [← hX, Set.ext_iff]
+  refine fun y => ⟨?_, ?_⟩
+  · rintro (hy|hy)
+    exact hy.left
+    exact hy ▸ x.prop
+  · rintro hy
+    by_cases hx : y = x.val
+    exact Or.inr hx
+    exact Or.inl ⟨hy, hx⟩
 
 /-- Exercise 3.6.11 -/
 theorem SetTheory.Set.two_to_two_iff {X Y:Set} (f: X → Y): Function.Injective f ↔
-    ∀ S ⊆ X, S.card = 2 → (image f S).card = 2 := by sorry
+    ∀ S ⊆ X, S.card = 2 → (image f S).card = 2 := by
+      constructor
+      · intro hf S hS hS_card
+        replace hS_card: S.has_card 2 := card_to_has_card (Nat.zero_ne_add_one _).symm hS_card
+        obtain ⟨x, y, hS_pair, hxy⟩ : ∃(x y: S), S = {x.val, y.val} ∧ x ≠ y := by
+          let x := nonempty_choose fun h => by
+            have := card_uniq hS_card (has_card_zero.mpr h)
+            contradiction
+          replace : (S \ {↑x}).has_card 1 := card_erase (Nat.le_succ _) hS_card x
+          let y := nonempty_choose fun h => by
+            have := card_uniq this (has_card_zero.mpr h)
+            contradiction
+          replace : ((S \ {↑x}) \ {↑y}) = ∅ := has_card_zero.mp <| card_erase (Nat.le_refl _) this y
+          replace := empty_union _ ▸ sdiff_of_singleton_mem this 
+            |>.symm |> sdiff_of_singleton_mem
+            |>.symm
+          replace : S = {↑x, ↑y} := by simp [Set.ext_iff, this, or_comm]
+          refine ⟨x, ⟨y.val, mem_sdiff _ _ _ |>.mp y.prop |>.left⟩, this, ?_⟩
+          replace := mem_singleton _ _ |>.eq ▸ (mem_sdiff _ _ _ |>.mp y.prop |>.right)
+          exact Subtype.coe_ne_coe.mp fun a ↦ this a.symm
+        rw [hS_pair,  image_pair (hS _ x.prop) (hS _ y.prop)]
+        refine has_card_to_card <| pair_has_card ?_
+        by_contra h
+        simp [coe_inj, hf.eq_iff, hxy] at h
+      intro hS x y h
+      by_cases hxy : x = y
+      · exact hxy
+      have : {x.val, y.val} ⊆ X := by
+        intro x' hx'
+        obtain rfl|rfl := mem_pair _ _ _ |>.mp hx'
+        exact x.prop
+        exact y.prop
+      specialize hS _ this (has_card_to_card <| pair_has_card <| Subtype.coe_ne_coe.mpr hxy)
+      rw [image_pair x.prop y.prop, h, pair_self] at hS
+      replace hS : ({↑(f y)}: Set).has_card 2 := card_to_has_card (Nat.zero_ne_add_one _).symm hS
+      replace hS := card_uniq (hS) (singleton_has_card _)
+      contradiction
+
+
+          
+
+
 
 /-- Exercise 3.6.12 -/
 def SetTheory.Set.Permutations (n: ℕ): Set := (Fin n ^ Fin n).specify (fun F ↦
